\section{Bài 5}

\subsection{Đề bài}

Chứng minh $XY = iZ$ bằng cách:
\begin{itemize}
    \item[(a)] Nhân ma trận.
    \item[(b)] Xét tác động của các toán tử trên $\ket{0}, \ket{1}$ .
\end{itemize}

\subsection{Lời giải}
\subsubsection{Phần (a)}
Ta có:
\[
X = 
\begin{bmatrix}
    0 & 1 \\
    1 & 0
\end{bmatrix},
Y = 
\begin{bmatrix}
    0 & -i \\
    i & 0
\end{bmatrix},
Z =
\begin{bmatrix}
    1 & 0 \\
    0 & -1
\end{bmatrix}
\]
\[
\Rightarrow
\begin{cases}
    XY = \begin{bmatrix}
        0 & 1 \\
        1 & 0
    \end{bmatrix}
    \begin{bmatrix}
        0 & -i \\
        i & 0
    \end{bmatrix}
    = 
    \begin{bmatrix}
        i & 0 \\
        0 & -i
    \end{bmatrix} \\
    iZ = i
    \begin{bmatrix}
        1 & 0 \\
        0 & -1
    \end{bmatrix}
    = 
    \begin{bmatrix}
        i & 0 \\
        0 & -i
    \end{bmatrix}   
\end{cases}
\]
$\Rightarrow XY = iZ = \begin{bmatrix} i & 0 \\ 0 & -i \end{bmatrix} \Rightarrow$ dpcm. 

\subsubsection{Phần (b)}
Ta có:
\begin{align*}
    X\ket{0} = \ket{1}&, X\ket{1} = \ket{0} \\
    Y\ket{0} = i\ket{1}&, Y\ket{1} = -i\ket{0} \\
    Z\ket{0} = \ket{0}&, Z\ket{1} = -\ket{1}
\end{align*}
Xét biểu thức sau:
\[
XY \ket{0} = X\left(Y\ket{0}\right) = X \left(i\ket{1}\right) = iX\ket{1} = i\ket{0} = i\left(Z\ket{0}\right) \Leftrightarrow XY\ket{0} = iZ\ket{0}.
\]
\[
XY \ket{1} = X\left(Y\ket{1}\right) = X \left(-i\ket{0}\right) = -iX\ket{0} = -i\ket{1} = i\left(Z\ket{1}\right) \Leftrightarrow XY\ket{1} = iZ\ket{1}.
\]
Vì $\left\{\ket{0}, \ket{1}\right\}$ là tập cơ sở nên $XY = iZ \Rightarrow$ dpcm.